src/axiomatic/Machine.v
@@ -28,65 +28,69 @@ Remove Hints plus_n_O.
 
 Section Operational. 
 
-Record configuration := 
-  { ts : IdentMap.t {lang:Language.t & lang.(Language.state)};
-    acts : list event ;
+Record execution := 
+  { acts : list event ;
     sb : event -> event -> Prop ; 
     rmw : event -> event -> Prop ; 
     rf : event -> event -> Prop ; 
     mo : event -> event -> Prop ; 
     sc : event -> event -> Prop }.
 
-Inductive mstep mc mc' e i : Prop :=
-  | silent (SILENT: e = None) 
-      (SAME_ACTS: acts mc = acts mc')
-      (SAME_SB: sb mc = sb mc') 
-      (SAME_RMW: rmw mc = rmw mc') 
-      (SAME_RF: rf mc = rf mc')
-      (SAME_MO: mo mc = mo mc') 
-      (SAME_SC: sc mc = sc mc')
+(* Definition Coherent_exec G :=
+  Coherent (acts G) (sb G) (rmw G) (rf G) (mo G) (sc G).
+ *)
+Record configuration := 
+  { ts : IdentMap.t {lang:Language.t & lang.(Language.state)};
+    exec : execution }.
+
+Inductive mstep G G' e i : Prop :=
+  | silent (SILENT: e = None) (SAME_EXEC: G' = G)
   | read a l v o 
       (EVENT: e = Some (ProgramEvent.read l v o)) 
       (LABa: lab a = Aload l v o) 
       (TIDa: thread a = i) 
-      (GSTEP: gstep (acts mc) (sb mc) (rmw mc) (rf mc) (mo mc) (sc mc)
-                    (acts mc') (sb mc') (rmw mc') (rf mc') (mo mc') (sc mc') a a)
-      (COH': Coherent (acts mc') (sb mc') (rmw mc') (rf mc') (mo mc') (sc mc'))
+      (GSTEP: gstep (acts G) (sb G) (rmw G) (rf G) (mo G) (sc G)
+                    (acts G') (sb G') (rmw G') (rf G') (mo G') (sc G') a a)
+      (COH': Coherent (acts G') (sb G') (rmw G') (rf G') (mo G') (sc G'))
   | write a l v o 
       (EVENT: e = Some (ProgramEvent.write l v o)) 
       (LABa: lab a = Astore l v o) 
       (TIDa: thread a = i) 
-      (GSTEP: gstep (acts mc) (sb mc) (rmw mc) (rf mc) (mo mc) (sc mc)
-                    (acts mc') (sb mc') (rmw mc') (rf mc') (mo mc') (sc mc') a a)
-      (COH': Coherent (acts mc') (sb mc') (rmw mc') (rf mc') (mo mc') (sc mc'))
+      (GSTEP: gstep (acts G) (sb G) (rmw G) (rf G) (mo G) (sc G)
+                    (acts G') (sb G') (rmw G') (rf G') (mo G') (sc G') a a)
+      (COH': Coherent (acts G') (sb G') (rmw G') (rf G') (mo G') (sc G'))
   | update a_r a_w l v_r v_w o_r o_w 
       (EVENT: e = Some (ProgramEvent.update l v_r v_w o_r o_w)) 
       (LABar: lab a_r = Aload l v_r o_r) (LABaw: lab a_w = Astore l v_w o_w) 
       (SC_IMPL_ACQ: is_sc a_w -> is_acq a_r)
       (TIDar: thread a_r = i) (TIDaw: thread a_w = i) 
-      mc_mid
-      (GSTEPr: gstep (acts mc) (sb mc) (rmw mc) (rf mc) (mo mc) (sc mc)
-           (acts mc_mid) (sb mc_mid) (rmw mc_mid) (rf mc_mid) (mo mc_mid) (sc mc_mid) a_r a_r)
-      (GSTEPw: gstep (acts mc_mid) (sb mc_mid) (rmw mc_mid) (rf mc_mid) (mo mc_mid) (sc mc_mid)
-                     (acts mc') (sb mc') (rmw mc') (rf mc') (mo mc') (sc mc') a_r a_w)
-      (COHmid: Coherent (acts mc_mid) (sb mc_mid) (rmw mc_mid) (rf mc_mid) (mo mc_mid) 
-                        (sc mc_mid))
-      (COH': Coherent (acts mc') (sb mc') (rmw mc') (rf mc') (mo mc') (sc mc'))
+      G_mid
+      (GSTEPr: gstep (acts G) (sb G) (rmw G) (rf G) (mo G) (sc G)
+           (acts G_mid) (sb G_mid) (rmw G_mid) (rf G_mid) (mo G_mid) (sc G_mid) a_r a_r)
+      (GSTEPw: gstep (acts G_mid) (sb G_mid) (rmw G_mid) (rf G_mid) (mo G_mid) (sc G_mid)
+                     (acts G') (sb G') (rmw G') (rf G') (mo G') (sc G') a_r a_w)
+      (COH': Coherent (acts G_mid) (sb G_mid) (rmw G_mid) (rf G_mid) (mo G_mid) (sc G_mid))
+      (COH': Coherent (acts G') (sb G') (rmw G') (rf G') (mo G') (sc G'))
   | fence a o_r o_w (EVENT: e = Some (ProgramEvent.fence o_r o_w)) 
       (LABa: lab a = Afence o_r o_w) 
       (TIDa: thread a = i) 
-      (GSTEP: gstep (acts mc) (sb mc) (rmw mc) (rf mc) (mo mc) (sc mc)
-                    (acts mc') (sb mc') (rmw mc') (rf mc') (mo mc') (sc mc') a a)
-      (COH': Coherent (acts mc') (sb mc') (rmw mc') (rf mc') (mo mc') (sc mc')).
+      (GSTEP: gstep (acts G) (sb G) (rmw G) (rf G) (mo G) (sc G)
+                    (acts G') (sb G') (rmw G') (rf G') (mo G') (sc G') a a)
+      (COH': Coherent (acts G') (sb G') (rmw G') (rf G') (mo G') (sc G'))
+  | syscall a ee (EVENT: e = Some (ProgramEvent.syscall ee)) 
+      (LABa: lab a = Afence Ordering.seqcst Ordering.seqcst) 
+      (TIDa: thread a = i) 
+      (GSTEP: gstep (acts G) (sb G) (rmw G) (rf G) (mo G) (sc G)
+                    (acts G') (sb G') (rmw G') (rf G') (mo G') (sc G') a a)
+      (COH': Coherent (acts G') (sb G') (rmw G') (rf G') (mo G') (sc G')).
 
 Inductive step mc mc' : Prop :=
 | step_intro  
     lang st st' i e
     (TID: IdentMap.find i (ts mc) = Some (existT _ lang st))
     (STATE: lang.(Language.step) e st st')
-    (MTS: ts mc' = IdentMap.add i (existT _ _ st') (ts mc))
-    (MSTEP: mstep mc mc' e (Some i))
-.
+    (MTS: ts mc' = IdentMap.add i (existT _ lang st') (ts mc))
+    (MSTEP: mstep (exec mc) (exec mc') e (Some i)).
 
 End Operational.
 
