src/axiomatic/GsimM.v
@@ -1,0 +1,1142 @@
+(******************************************************************************)
+(** * The axiomatic machine simulates the promise-free machine  *)
+(******************************************************************************)
+
+Require Import Classical List Relations Peano_dec.
+Require Import Hahn.
+Require Import sflib.
+Require Import paco.
+
+Require Import Axioms.
+Require Import Basic.
+Require Import Language.
+Require Import Event.
+Require Import Time.
+Require Import Configuration.
+Require Import View.
+Require Import Cell.
+Require Import Memory.
+Require Import Thread.
+Require Import TView.
+
+Require Import Gevents.
+Require Import model.
+Require Import Gstep GstepRead GstepWrite GstepFence GstepOther.
+Require Import Machine.
+Require Import SimRel SimPreservation.
+Require Import SmallStep.
+
+
+Set Implicit Arguments.
+Remove Hints plus_n_O.
+
+Require Import Setoid Permutation.
+
+Hint Resolve gstep_wf gstep_inc coh_wf.
+
+Definition GMsim op_st ax_st :=
+  << COH: Coherent (acts (exec ax_st)) (sb (exec ax_st)) (rmw (exec ax_st)) 
+    (rf (exec ax_st)) (mo (exec ax_st)) (sc (exec ax_st)) >> /\
+  << WF_OP_ST: Configuration.wf op_st >> /\
+  << NO_PROMISES: forall i foo local 
+        (TID: IdentMap.find i (Configuration.threads op_st) = Some (foo, local)),
+         local.(Local.promises) = Memory.bot>> /\
+  << STATES: (ts ax_st) = IdentMap.map fst (Configuration.threads op_st) >>/\
+  << TIME: exists f_from f_to, sim_time (Configuration.threads op_st)
+     (Configuration.sc op_st) (Configuration.memory op_st) (exec ax_st) f_from f_to >>.
+
+Definition get_program_event (e:ThreadEvent.t) : option ProgramEvent.t :=
+  match e with
+  |ThreadEvent.read loc _ val _ ord => Some (ProgramEvent.read loc val ord)
+  |ThreadEvent.write loc _ _ val _ ord => Some (ProgramEvent.write loc val ord)
+  |ThreadEvent.update loc _ _ valr valw _ _ ordr ordw => 
+      Some (ProgramEvent.update loc valr valw ordr ordw)
+  |ThreadEvent.fence ordr ordw => Some (ProgramEvent.fence ordr ordw)
+  |ThreadEvent.syscall ev => Some (ProgramEvent.syscall ev)
+  | _ => None
+  end.
+
+Lemma GMsim_helper tss G ths sc_map mem 
+  (COH: Coherent (acts G) (sb G) (rmw G) (rf G) (mo G) (sc G))
+  (WF_OP_ST: Configuration.wf (Configuration.mk ths sc_map mem))
+  (NO_PROMISES: forall i foo local (TID: IdentMap.find i ths = Some (foo, local)),
+         local.(Local.promises) = Memory.bot)
+  (STATES: tss = IdentMap.map fst ths)
+  f_from f_to (TIME: sim_time ths sc_map mem G f_from f_to)
+  tid e lang st lc st' lc' ths' sc_map' mem' 
+  (THS2: ths' = IdentMap.add tid (existT Language.state lang st', lc') ths) 
+  (TID: IdentMap.find tid ths = Some (existT Language.state lang st, lc))
+  (STEP: Thread.step e (Thread.mk lang st lc sc_map mem) 
+    (Thread.mk lang st' lc' sc_map' mem'))
+  (PFREE: ThreadEvent.is_promising e = None)
+  G' (MSTEP: mstep G G' (get_program_event e) (Some tid))
+  f_from' (F_FROM: forall b, In b (acts G) -> f_from' b = f_from b)
+  f_to' (F_TO: forall b, In b (acts G) -> f_to' b = f_to b)
+  (MONOTONE: monotone (mo G') f_to')
+  (SIM_TVIEW: forall foo local
+        (TID: IdentMap.find tid ths' = Some (foo,local)),
+        sim_tview f_to' (acts G') (sb G') (rmw G') (rf G') (sc G') 
+                        local.(Local.tview) (Some tid))
+  (SIM_SC_MAP: forall l, max_value f_to' (S_tm (acts G') (sb G') (rmw G') (rf G') l) 
+                                     (LocFun.find l sc_map'))
+  (SIM_MEM: sim_mem f_from' f_to' (acts G') (sb G') (rmw G') (rf G') (sc G') mem'):
+  exists ax_st', step {| ts:=tss; exec:=G |}  ax_st' /\ 
+    GMsim (Configuration.mk ths' sc_map' mem')  ax_st'.
+Proof.
+unfold GMsim in *; desc.
+rewrite THS2.
+destruct STEP; try by destruct STEP; ins.
+eexists  {| ts:=  IdentMap.add tid (existT _ _ st') tss; exec:= G' |}; splits.
+- inv STEP. 
+  all: econstructor; ins; try edone.
+  all: try rewrite STATES.
+  all: rewrite IdentMap.Facts.map_o; unfold option_map; ins; desf; eauto.
+- by destruct MSTEP; subst; eauto.
+- eapply Configuration.step_future; eauto using no_promises_consistent.
+  econs; eauto.
+  eexists; splits; try econs.
+  by eapply Progress.program_step_promise; eauto.
+- intro; simpl; rewrite IdentMap.gsspec; ins; desf; simpl.
+  by eapply Progress.program_step_promise; eauto.
+  by eapply NO_PROMISES; eauto.
+- ins; rewrite IdentMap.map_add; simpl; by rewrite STATES.
+- unfold sim_time in *; ins; desc.
+  eexists f_from',f_to'; splits; eauto; ins.
+  rewrite IdentMap.gsspec in TID0; desf; ins; simpl.
+  eapply SIM_TVIEW; eauto using UsualFMapPositive.UsualPositiveMap'.gss.
+  apply SIM_TVIEW0 in TID0.
+  inv STEP; inv MSTEP; try by unfold get_program_event in *; ins; desf.
+  by eapply sim_tview_other_threads_silent; eauto.
+  all: eapply sim_tview_other_threads; eauto 2.
+  all: try eapply sim_tview_other_threads; eauto 2.
+  all: try intro; subst; eauto.
+  all: congruence.
+Qed.
+
+Require Import Omega.
+
+Lemma fresh_id (acts: list event) tid lb:
+  exists a, << THREAD_ID: thread a = tid >> /\ <<LABEL: lab a = lb >> /\ 
+  <<FRESH: ~ In a acts >>.
+Proof.
+eexists (Event (1 + fold_right (fun x c => S (id x + c)) 0 acts) _ _); splits; try by simpl; eauto.
+generalize 1; generalize 0; induction acts; ins.
+intro; desf; desf; eauto.
+destruct a; ins; desf; omega.
+rewrite <- plus_Sn_m, Const.add_assoc in H; eapply IHacts; eauto.
+Qed.
+
+(******************************************************************************)
+(** * Lemmas for silent step  *)
+(******************************************************************************)
+
+Lemma GMsim_silent ts G op_st tid lang st1 st2 lc2 
+  (SIM: GMsim op_st {| ts:= ts; exec:= G |})
+  (STATE: Language.step lang None st1 st2)
+  (TID: IdentMap.find tid (Configuration.threads op_st) =
+      Some (existT (fun lang : Language.t => Language.state lang) lang st1, lc2)):
+  exists ax_st', step {| ts:= ts; exec:= G |} ax_st' /\
+      GMsim (Configuration.mk 
+        (IdentMap.add tid (existT Language.state lang st2, lc2) 
+          (Configuration.threads op_st))
+        (Configuration.sc op_st)
+        (Configuration.memory op_st)) ax_st'.
+Proof.
+destruct op_st; ins.
+unfold GMsim in *; desc; ins.
+unfold sim_time in *; desc.
+eapply GMsim_helper with (e:=ThreadEvent.silent) (tid:=tid); eauto.
+
+econs; ins; eauto.
+econs; eauto.
+ins; eapply SIM_TVIEW.
+rewrite IdentMap.gsspec in TID0; desf; ins; simpl; eauto.
+by exfalso; auto.
+Qed.
+
+(******************************************************************************)
+(** * Lemmas about well-formedness of the new graph  *)
+(******************************************************************************)
+
+Lemma wf_new_acts acts sb rmw rf mo sc (WF: Wf acts sb rmw rf mo sc)
+  a (FRESH: ~ In a acts) (PROPER: is_proper a): WfACTS (a :: acts).
+Proof.
+cdes WF.
+unfold WfACTS in *; desc; splits.
+by intros; right; eauto.
+by intros; destruct IN; desf; eauto.
+Qed.
+
+Lemma wf_new_sb acts sb rmw rf mo sc (WF: Wf acts sb rmw rf mo sc)
+  a (FRESH: ~ In a acts) (PROPER: is_proper a): WfSB (a :: acts) (sb +++ sb_ext acts a).
+Proof.
+cdes WF.
+unfold WfSB in *; desc; splits; ins.
+all: try by destruct SB; unfold sb_ext, seq, eqv_rel in *; desc; subst; eauto.
+- destruct SB; eauto. 
+  unfold sb_ext, seq, eqv_rel, init_pair in *; desf; subst; eauto.
+  left; splits; eauto; eapply thread_proper; eauto.
+- unfold sb_ext, union, seq, eqv_rel, init_pair in *; desf; subst; eauto.
+  unfold WfACTS in *; desc; eauto 10.
+- intros x A; red in A; desf; unfold sb_ext, seq, eqv_rel in *; desf; eauto.
+- intros x y z A B.
+  unfold sb_ext, union, seq, eqv_rel in *; desf; eauto.
+  by exfalso; apply FRESH; eauto.
+  by exfalso; apply FRESH; eauto.
+  right; eexists; splits; eauto.
+  exists z; splits; eauto.
+  apply SB_TID in A; desf.
+  left; congruence.
+  right; red in A; desc; eauto.
+  exfalso.
+  apply SB_TID in A; desf.
+  eapply init_proper_thread; eauto.
+  eapply proper_non_init; red in A; desc; eauto.
+- desf; unfold sb_ext, seq, eqv_rel, union; eauto 10.
+  exploit SB_TOT; eauto; ins; desf; eauto.
+Qed.
+
+Lemma wf_new_rmw acts sb rmw rf mo sc (WF: Wf acts sb rmw rf mo sc)
+  a (FRESH: ~ In a acts) (PROPER: is_proper a): WfRMW (sb +++ sb_ext acts a) rmw.
+Proof.
+cdes WF.
+unfold WfRMW in *; desc; splits; ins.
+- by left; eauto.
+- destruct SB.
+  left; eapply RMW_SBI; eauto.
+  unfold sb_ext, seq, eqv_rel in *; desc; subst.
+  by exfalso; apply FRESH; eapply rmw_actb; eauto.
+- destruct SB.
+  left; eapply RMW_SBI'; eauto.
+  unfold sb_ext, seq, eqv_rel in *; desc; subst.
+  right; exists b; splits; eauto_red using rmw_actb.
+  exists c; splits; eauto.
+  destruct H0.
+  assert (RMW' := RMW).
+  apply RMW_SB in RMW.
+  apply WF_SB in RMW.
+  desf.
+  by left; congruence.
+  apply RMW_DOMa in RMW'.
+  by exfalso; eapply read_non_write; red in RMW; desc; eauto using init_is_write.
+  by exfalso; eapply read_non_write with (a:=z); eauto using init_is_write.
+Qed.
+
+Lemma wf_new_rf acts sb rmw rf mo sc (WF: Wf acts sb rmw rf mo sc)
+  a (FRESH: ~ In a acts) (PROPER: is_proper a)
+  (NON_READ: ~ is_read a) : WfRF (a :: acts) rf.
+Proof.
+cdes WF.
+unfold WfRF in *; desc; splits; ins; eauto.
+exploit RF_TOT; eauto; desf.
+Qed.
+
+Lemma wf_new_mo acts sb rmw rf mo sc (WF: Wf acts sb rmw rf mo sc)
+  a (FRESH: ~ In a acts) (PROPER: is_proper a)
+  (NON_WRITE: ~ is_write a) : WfMO (a :: acts) mo.
+Proof.
+cdes WF.
+unfold WfMO in *; desc; splits; ins; eauto.
+red; ins; desf.
+all: try by exfalso; eapply read_non_write; eauto.
+eapply MO_TOT; splits; eauto.
+Qed.
+
+Lemma wf_new_sc acts sb rmw rf mo sc (WF: Wf acts sb rmw rf mo sc)
+  a (FRESH: ~ In a acts) (PROPER: is_proper a): WfSC (a :: acts) (sc +++ sc_ext acts a).
+Proof.
+cdes WF.
+unfold WfSC in *; desc; splits; ins; eauto.
+all: try unfold union, sc_ext in *; desf; eauto.
+- intros x A; desf; eauto.
+- intros x y z A B; desf; eauto 10.
+  exfalso; eapply FRESH; eauto.
+- red; ins; desf; eauto 8.
+  assert (sc a0 b \/ sc b a0).
+    eauto.
+  desf; eauto.
+Qed.
+
+(******************************************************************************)
+(** * Lemmas for read step  *)
+(******************************************************************************)
+
+Definition new_G_read G a b :=
+{| acts:=(a :: acts G); sb:=(sb G +++ sb_ext (acts G) a);
+           rmw:=(rmw G) ; rf:=(rf G +++ singl_rel b a); mo:= (mo G);
+           sc:=(Machine.sc G +++ sc_ext (acts G) a) |}.
+
+Lemma exists_gstep_read acts sb rmw rf mo sc a 
+  (WF: Wf acts sb rmw rf mo sc)
+  (FRESH: ~ In a acts) (PROPER: is_proper a) (READa: is_read a)
+  b (INb: In b acts) (WRITEb: is_write b) 
+  (LOC: exists l, loc b = Some l /\ loc a = Some l) (VAL: val b = val a):
+  gstep acts sb rmw rf mo sc 
+      (a :: acts) (sb +++ sb_ext acts a)
+      rmw (rf +++ singl_rel b a) mo (sc +++ sc_ext acts a) a a.
+Proof.
+red; splits; eauto.
+by unfold sb_ext, union, eqv_rel, seq; eauto 8.
+by red; eauto.
+by unfold sc_ext, union; eauto.
+by red; unfold inclusion, union; splits; ins; eauto.
+red; splits.
+- eby eapply wf_new_acts.
+- eby eapply wf_new_sb.
+- eby eapply wf_new_rmw.
+- cdes WF; unfold WfRF in *; desc; splits; ins.
+  all: try unfold union, singl_rel in *; desf; eauto.
+  all: try by exfalso; apply FRESH; eauto.
+  exploit RF_TOT; eauto; ins; desc; eauto.
+- eapply wf_new_mo; eauto 2 with acts.
+- eby eapply wf_new_sc.
+Qed.
+
+Lemma new_G_read_NoPromises acts sb rmw rf mo sc acts' sb' rmw' rf' mo' sc'
+  (COH: Coherent acts sb rmw rf mo sc)  
+  a (GSTEP: gstep acts sb rmw rf mo sc acts' sb' rmw' rf' mo' sc' a a)
+  b (NEQ: b <> a) :
+  NoPromises sb' (rf +++ (singl_rel b a)) sc'.
+Proof.
+cdes GSTEP; cdes COH.
+exploit gstep_sb; eauto.
+exploit gstep_sc; eauto.
+intros Usb Usc; rewrite Usb, Usc.
+red; rewrite !unionA, (unionAC _ rf), 2!(unionAC _ sc), <- 2!unionA, unionC.
+assert (MAX: forall x y,
+  (sb_ext acts a +++ (singl_rel b a +++ sc_ext acts a)) x y -> y = a).
+  by intros x y R; unfold sb_ext, singl_rel, sc_ext, seq, eqv_rel, union in R; desf.
+apply acyclic_decomp_u_1; try done.
+- ins; apply MAX in R; subst.
+  unfold union in R'; desf;
+  eapply FRESH; [eapply sb_acta| eapply rf_acta| eapply sc_acta]; edone.
+- red; red; ins.
+  eapply cycle_disj; cycle 1; try edone.
+  ins; apply MAX in R; subst.
+  unfold sb_ext, singl_rel, sc_ext, seq, eqv_rel, union in R'; desf; auto.
+Qed.
+
+Lemma new_G_read_coherent 
+  acts sb rmw rf mo sc sc_map memory tview a
+  (COH: Coherent acts sb rmw rf mo sc)
+  f_from f_to (MONOTONE: monotone mo f_to)
+  (SIM_TVIEW: sim_tview f_to acts sb rmw rf sc tview (thread a))
+  (SIM_SC_MAP: forall l, max_value f_to (S_tm acts sb rmw rf l) (LocFun.find l sc_map))
+  (SIM_MEM: sim_mem f_from f_to acts sb rmw rf sc memory)
+  l v released o from b
+  (READABLE: TView.readable tview l (f_to b) released o)
+  (INb: In b acts) (WRITEb: is_write b) (LOCb: loc b = Some l)
+  (HELPERb: sim_mem_helper f_to acts sb rmw rf sc b from v (View.unwrap released))
+  (LABEL: lab a = Aload l v o)
+  (FRESH: ~ In a acts)
+  acts' sb' rmw' rf' mo' sc'
+  (NEW_G: new_G_read {| acts:=acts; sb:=sb; rmw:=rmw; rf:=rf; mo:=mo; sc:=sc |}
+   a b = {| acts:=acts'; sb:=sb'; rmw:=rmw'; rf:=rf'; mo:=mo'; sc:=sc' |})
+  (GSTEP: gstep acts sb rmw rf mo sc 
+               acts' sb' rmw' rf' mo' sc' a a):
+  Coherent acts' sb' rmw' rf' mo' sc'.
+Proof.
+unfold new_G_read in *; ins; desf.
+
+exploit gstep_hb_read; eauto.
+right; edone.
+intro HB.
+ 
+assert (forall x y (MOxy: mo' x y), In y acts).
+  ins; eapply mo_actb; eauto.
+
+assert (forall x y (MOxy: mo' x y), is_write y).
+  ins; eapply mo_domb; eauto. 
+
+assert (forall x y (MOxy: mo' x y) (LOC: loc x = Some l), (loc y = Some l)).
+  ins; eapply loceq_mo in MOxy; eauto.
+  rewrite <- MOxy; done.
+
+destruct READABLE; desc.
+red in SIM_TVIEW; desc.
+red in CUR; desc.
+specialize (CUR_UR l).
+specialize (CUR_RW l).
+specialize (CUR_SC l).
+
+cdes COH; red; splits; eauto.
+- red; ins; destruct RF as [RF1|RF2].
+  by eapply Crmw; eauto.
+  by red in RF2; desc; desf; eapply rmw_acta in RMW; eauto.
+- red; ins; eapply gstep_hb_a in HB0; try edone.
+  destruct RF; unfold singl_rel in *; desf; eauto 2.
+  eby apply FRESH; eapply hb_acta.
+  eby intro; subst; apply FRESH; eapply mo_acta.
+- red; ins; eapply gstep_hb_a in HB0; eauto 2.
+  eby intro; subst; apply FRESH; eapply mo_acta.
+- red; ins; destruct RF; unfold singl_rel in *; desf.
+  eapply gstep_hb_a in HB0; eauto 2.
+  eby intro; subst; apply FRESH; eapply rf_actb.
+  apply HB in HB0; destruct HB0 as [?|[c[B[C|D]]]]; 
+  unfold sb_ext, eqv_rel, seq in *; desc; try subst z z0.
+  eby apply FRESH; eapply hb_actb.
+  eby eapply max_value_le; eauto; repeat (eexists; splits; eauto).
+  eby eapply Coherent_urr_rel; eauto; repeat (eexists; splits; eauto).
+- red; ins; destruct RF; unfold singl_rel in *; desf; try eby eapply max_elt_hb.
+  apply HB in HB0; clear HB.
+  destruct RF'; unfold singl_rel in *; desf; destruct HB0 as [?|HB0]; eauto 2.
+  by apply FRESH; eapply rf_actb; try edone;
+    unfold union, sb_ext, seq, eqv_rel in *; desf; subst; eauto.
+  eby apply FRESH; eapply hb_actb.
+  destruct HB0 as [d A];
+  unfold union, sb_ext, eqv_rel, seq in *; desc.
+  assert (rwr acts sb rmw' rf sc l b0 d).
+    by right; repeat (eexists; splits; eauto).
+  destruct A0; desc; subst z z0.
+  * eapply max_value_le with (tm:=View.rlx (TView.cur tview)); eauto.
+    by red in RLX; rewrite LABEL in *; ins; auto.
+    by exists d; repeat (eexists; splits; eauto).
+  * eby eapply Coherent_rwr_rel.
+- red; ins; destruct RF; unfold singl_rel in *; desf; try eby eapply max_elt_hb.
+  eapply gstep_hb_a in HB0; try edone; cycle 1.
+  eby intro; subst; eapply max_elt_hb.
+  destruct RF'; desf.
+  * eapply gstep_hb_a in HB1; eauto 2.
+    eby intro; subst; eapply FRESH; eapply rf_actb.
+  * apply HB in HB1; clear HB.
+    destruct HB1 as [?|HB1].
+    eby apply FRESH; eapply hb_actb.
+    destruct HB1 as [e A];
+    unfold union, sb_ext, eqv_rel, seq in *; desc.
+    assert (urr acts sb rmw' rf sc l b0 e).
+      by clear A0; unfold urr, rfhbsc_opt, seq, eqv_rel, clos_refl in *; desf; eauto 25. 
+    destruct A0; desc; subst z z0.
+    + eapply max_value_le; eauto.
+      by exists e; repeat (eexists; splits; eauto).
+    + eby eapply Coherent_urr_rel.
+- red; ins; destruct RF; unfold singl_rel in *; 
+  desf; eauto 2; eby eapply max_elt_rmw.
+- red; ins.
+  assert (RFHBF_: b0 = d \/
+          (exists c, clos_refl rf b0 c /\ hb acts sb rmw' rf c d /\ is_sc_fence d)).
+    destruct RFHBF as [X|[c [RF' [HB' F]]]]; auto.
+    right; exists c; splits; try edone.
+    destruct RF' as [?|[X|Y]]; unfold singl_rel in *; desc; subst; try by econs.
+    eby exfalso; eapply max_elt_hb.
+    eapply gstep_hb_a in HB'; try edone.
+    eby intro; subst; eapply max_elt_sc.
+  clear RFHBF.
+  destruct SC as [SC|X]; cycle 1; unfold sc_ext in *; desc; subst.
+  by unfold is_sc_wf in *; destruct a as [??[]]; desf; ins.
+  apply HB in HB0; clear HB.
+  destruct HB0 as [X|HB0].
+  destruct RF; unfold singl_rel in *; desc; subst; eauto 2.
+  eby apply FRESH; eapply hb_actb.
+  assert (f=a).
+   by unfold union, sb_ext, seq, eqv_rel, singl_rel in *; desf.
+  subst f.
+  destruct RF as [?|RF]; subst.
+  by eapply FRESH, rf_actb; eauto.
+  red in RF; desc; subst a0.
+  unfold union, sb_ext, seq, eqv_rel, singl_rel in *.
+  assert (rfhbsc_opt acts sb rmw' rf l b0 d).
+   by clear HB0; red; unfold seq, eqv_rel, clos_refl in *; desf; eauto 20.
+  destruct HB0 as [z HB0].
+  assert (SC':=SC).
+  eapply sc_domb in SC'; try edone.
+  destruct SC' as [Ef|Ew].
+  * assert (urr acts sb rmw' rf sc l b0 z).
+    by unfold urr, seq, eqv_rel, clos_refl in *; desf; eauto 10.
+    destruct HB0 as [HB0 [SB|REL']]; desc; subst z1 z0.
+    eapply max_value_le; eauto.
+    exists z,z; splits; eauto.
+    by repeat (eexists; splits; eauto).
+    eby eapply Coherent_urr_rel.
+  * assert (is_write e).
+     by destruct e as [??[]]; ins.
+    assert (Ordering.le Ordering.seqcst o).
+     by exploit SCread; try edone; intro SCa; red in SCa; destruct (lab a); ins; desf.
+    assert (scr acts sb rmw' rf sc l b0 z).
+     by right; unfold seq, eqv_rel, clos_refl in *; desf; eauto 10.
+    destruct HB0 as [HB0 [SB|REL']]; desc; subst z1 z0.
+    + eapply max_value_le with (tm:=View.sc (TView.cur tview)); eauto.
+      exists z,z; splits; eauto.
+      repeat (eexists; splits; eauto).
+    + red in HELPERb; desc; red in SIMMSG; desc; specialize (SC0 l).
+      eapply max_value_le with (tm:=View.sc (View.unwrap released)); eauto; ins.
+      exists z; splits; eauto.
+
+- red; ins.
+  assert (RFHBF_: b0 = d \/
+        (exists c, clos_refl rf b0 c /\ hb acts sb rmw' rf c d /\ is_sc_fence d)).
+    destruct RFHBF as [X|[c [RF' [HB' F]]]]; auto.
+    right; exists c; splits; try edone.
+    destruct RF' as [?|[X|Y]]; unfold singl_rel in *; desc; subst; try by econs.
+    eby exfalso; eapply max_elt_hb.
+    eapply gstep_hb_a in HB'; eauto 2.
+    intro; subst; eapply max_elt_sc; eauto.
+  clear RFHBF.
+  destruct SC as [SC|]; cycle 1; unfold sc_ext in *; desc; subst.
+  by unfold is_sc_wf in *; destruct a as [??[]]; desf; ins.
+  destruct HB0 as [|HB0]; subst; eauto 3.
+  desc; apply HB in HB0; clear HB.
+  destruct HB0 as [|HB0]; eauto 4.
+  assert (a0=a); subst.
+    by unfold union, sb_ext, seq, eqv_rel, singl_rel in *; desf; eauto.
+  eapply mo_doma in MO; try edone.
+  by destruct a as [??[]]; ins.
+- eapply new_G_read_NoPromises; try edone.
+  by intro; subst; eauto with acts.
+Qed.
+
+Lemma GMsim_read ts G tid lang st1 st2 lc1 lc2 threads sc_map mem
+  (SIM: GMsim (Configuration.mk threads sc_map mem) {| ts:= ts; exec:= G |})
+  (TID: IdentMap.find tid threads =
+        Some (existT (fun lang : Language.t => Language.state lang) lang st1, lc1))
+  l to v released o 
+  (STATE: Language.step lang (Some (ProgramEvent.read l v o)) st1 st2)
+  (LOCAL: Local.read_step lc1 mem l to v released o lc2):
+  exists ax_st', step {| ts:= ts; exec:= G |} ax_st' /\
+    GMsim (Configuration.mk (IdentMap.add tid (existT Language.state lang st2, lc2)
+                                 threads) sc_map mem)
+ ax_st'.
+Proof.
+unfold GMsim in *; desc; ins.
+unfold sim_time in *; desc.
+assert (LOCAL':=LOCAL).
+destruct LOCAL'; ins; subst.
+assert (SIM_MEM':= SIM_MEM).
+specialize (SIM_MEM' l); desc.
+specialize (SIMCELL to from v released GET); desc.
+
+generalize (fresh_id (acts G) (Some tid) (Aload l v o)); intro; desc.
+
+exploit exists_gstep_read; eauto with acts.
+by red; eauto.
+by exists l; splits; eauto with acts; unfold loc; desf.
+by red in SIMCELL4; desc; rewrite <- VAL; unfold val; desf.
+intro GSTEP.
+
+eapply GMsim_helper with 
+  (e:=ThreadEvent.read l to v released o) 
+  (tid:=tid)  
+  (G':= new_G_read G a b); eauto.
+- by red; eauto.
+- eapply read; eauto.
+  unfold get_program_event; eauto.
+  eapply new_G_read_coherent; eauto.
+  by rewrite THREAD_ID; eauto.
+  by rewrite SIMCELL3; eauto.
+- ins.
+  assert (LAB: exists o, lab b = Astore l v o); desc.
+    red in SIMCELL4; desc.
+    unfold Gevents.loc, is_write, val, lab in *.
+    destruct b as [??[]]; ins; desf; eauto.
+  exploit tview_step_read; eauto.
+  * by right; red; eauto.
+  * by apply SIMCELL4; rewrite THREAD_ID; eauto.
+  * by rewrite THREAD_ID in *; eapply SIM_TVIEW; eauto.
+  * rewrite IdentMap.gsspec in TID0; desf; ins.
+    eby rewrite THREAD_ID in *.
+    eby exfalso.
+- ins; eapply max_value_same_set; try edone.
+  by ins; rewrite gstep_S_tm_other; eauto with acts.
+- eapply memory_step_nonwrite; eauto.
+  eapply new_G_read_coherent; eauto.
+  rewrite THREAD_ID in *; eauto.
+  by rewrite SIMCELL3; eauto.
+  by eauto 3 with acts.
+Qed.
+
+(******************************************************************************)
+(** * Lemmas for write step  *)
+(******************************************************************************)
+
+Definition new_mo acts f_to a to:=
+  (fun x y => y = a /\ In x acts /\ is_write x /\ 
+    loc x = loc a /\ Time.lt (f_to x) to)  \2/ 
+  (fun x y => x = a /\ In y acts /\ is_write y /\ 
+    loc y = loc a /\ Time.lt to (f_to y)).
+
+Lemma wf_new_mo_write acts sb rmw rf mo sc (WF: Wf acts sb rmw rf mo sc)
+  a (FRESH: ~ In a acts) (PROPER: is_proper a) (WRITE: is_write a)
+  f_to to (MON: monotone mo f_to) 
+  (NEQ: forall b, In b acts /\ is_write b /\ loc b = loc a -> f_to b <> to):
+  WfMO (a :: acts) (mo +++ new_mo acts f_to a to).
+Proof.
+cdes WF; cdes WF_MO.
+unfold new_mo, union.
+red; splits.
+- ins; desf; eauto_red using mo_acta.
+- ins; desf; eauto_red using mo_actb.
+- ins; desf; eauto_red using mo_doma.
+- ins; desf; eauto_red using mo_domb.
+- ins; desf; eauto.
+  all: eapply write_has_location in MO1; desc; exists l; split; congruence.
+- red; ins; desf; eauto.
+- red; ins; desf; eauto.
+  all: try eby exfalso; apply FRESH; eapply mo_acta.
+  all: try eby exfalso; apply FRESH; eapply mo_actb.
+  all: try eby exfalso; eapply Time.lt_strorder, Time.lt_strorder.
+  * assert (Time.lt to (f_to z)).
+    eapply MON in H0.
+    eby eapply Time.lt_strorder.
+    right; right; splits; eauto.
+    specialize (MO_LOC y z H0); desc; congruence.
+  * assert (Time.lt (f_to x) to).
+    eapply MON in H.
+    eby eapply Time.lt_strorder.
+    right; left; splits; eauto.
+    specialize (MO_LOC x y H); desc; congruence.
+  * assert (Time.lt (f_to x) (f_to z)).
+    eby eapply Time.lt_strorder.
+    left; splits; eauto.
+    eapply write_has_location in WRITE; desc.
+    eapply wf_mo_tot with (l:=l); eauto; try congruence.
+    intro MO.
+    eapply MON in MO.
+    eby eapply Time.lt_strorder,Time.lt_strorder.
+    intro; subst.
+    eby eapply Time.lt_strorder.
+- assert (L: forall c, In c acts /\ is_write c /\ loc c = loc a -> 
+    Time.lt (f_to c) to \/ Time.lt to (f_to c)).
+    ins; destruct (Time.le_lt_dec (f_to c) to); auto.
+    rewrite Time.le_lteq in *; desf; auto.
+    eby edestruct NEQ.
+  unfold is_total in *; ins; desf; rewrite IWa1,IWb1 in *.
+  * destruct (L a0); eauto 10.
+  * destruct (L b); eauto 10.
+  * by exploit (MO_TOT l a0); eauto; ins; desf; eauto.
+Qed.
+
+Lemma new_f_to_monotone acts sb rmw rf mo sc (WF: Wf acts sb rmw rf mo sc)
+f_to a to (MON: monotone mo f_to) 
+(FRESH: ~ In a acts) (PROPER: is_proper a) (WRITE: is_write a)
+  (NEQ: forall b, In b acts /\ is_write b /\ loc b = loc a -> f_to b <> to):
+monotone (mo +++ new_mo acts f_to a to) (upd f_to a to).
+Proof.
+unfold monotone, upd, union, new_mo in *; ins; desf.
+eby exfalso; desf; cdes WF; eapply WF_MO.
+all: desf; eauto; try edone.
+eby exfalso; apply FRESH; eapply mo_acta.
+eby exfalso; apply FRESH; eapply mo_actb.
+Qed.
+
+Definition new_G_write G a f_to to :=
+{| acts:=(a :: acts G); sb:=(sb G +++ sb_ext (acts G) a);
+           rmw:=(rmw G) ; rf:=(rf G); mo:= (mo G) +++ new_mo (acts G) f_to a to;
+           sc:=(Machine.sc G +++ sc_ext (acts G) a) |}.
+
+Lemma exists_gstep_write acts sb rmw rf mo sc a 
+  (WF: Wf acts sb rmw rf mo sc)
+  (FRESH: ~ In a acts) (PROPER: is_proper a) (WRITEa: is_write a)
+  f_to to (WF_MO': WfMO (a :: acts) (mo +++ new_mo acts f_to a to)):
+  gstep acts sb rmw rf mo sc 
+      (a :: acts) (sb +++ sb_ext acts a)
+      rmw rf (mo +++ new_mo acts f_to a to) (sc +++ sc_ext acts a) a a.
+Proof.
+red; splits; eauto.
+by unfold sb_ext, union, eqv_rel, seq; eauto 8.
+by red; eauto.
+by unfold sc_ext, union; eauto.
+by red; unfold inclusion, union; splits; ins; eauto.
+red; splits; try done.
+- eby eapply wf_new_acts.
+- eby eapply wf_new_sb.
+- eby eapply wf_new_rmw.
+- eapply wf_new_rf; eauto 2 with acts.
+- eby eapply wf_new_sc.
+Qed.
+
+Lemma new_G_non_read_NoPromises acts sb rmw rf mo sc acts' sb' rmw' rf' mo' sc'
+  (COH: Coherent acts sb rmw rf mo sc)  
+  a (GSTEP: gstep acts sb rmw rf mo sc acts' sb' rmw' rf' mo' sc' a a):
+  NoPromises sb' rf sc'.
+Proof.
+cdes GSTEP; cdes COH.
+exploit gstep_sb; eauto.
+exploit gstep_sc; eauto.
+intros Usb Usc; rewrite Usb, Usc.
+red; rewrite !unionA, (unionAC _ rf), (unionAC _ sc), <- 2!unionA, unionC.
+assert (MAX: forall x y,
+  (sb_ext acts a +++ sc_ext acts a) x y -> y = a).
+  by intros x y R; unfold sb_ext, singl_rel, sc_ext, seq, eqv_rel, union in R; desf.
+apply acyclic_decomp_u_1; try done.
+- ins; apply MAX in R; subst.
+  unfold union in R'; desf;
+  eapply FRESH; [eapply sb_acta| eapply rf_acta| eapply sc_acta]; edone.
+- red; red; ins.
+  eapply cycle_disj; cycle 1; try edone.
+  ins; apply MAX in R; subst.
+  unfold sb_ext, singl_rel, sc_ext, seq, eqv_rel, union in R'; desf; auto.
+Qed.
+
+Lemma new_G_write_coherent 
+  acts sb rmw rf mo sc sc_map memory tview a
+  (COH: Coherent acts sb rmw rf mo sc)
+  f_from f_to (MONOTONE: monotone mo f_to)
+  (SIM_TVIEW: sim_tview f_to acts sb rmw rf sc tview (thread a))
+  (SIM_SC_MAP: forall l, max_value f_to (S_tm acts sb rmw rf l) (LocFun.find l sc_map))
+  (SIM_MEM: sim_mem f_from f_to acts sb rmw rf sc memory)
+  l v o to
+  (NEW_TO: forall x, In x acts /\ is_write x /\ loc x = Some l /\ 
+            Time.lt (f_from x) to /\ Time.le to (f_to x) -> False)
+  (WRITABLE: TView.writable tview sc_map l to o)
+  (LABEL: lab a = Astore l v o)
+  (FRESH: ~ In a acts)
+  acts' sb' rmw' rf' mo' sc' 
+  (NEW_MO: mo' = mo +++ new_mo acts f_to a to)
+  (NEW_G: new_G_write {| acts:=acts; sb:=sb; rmw:=rmw; rf:=rf; mo:=mo; sc:=sc |}
+   a f_to to = {| acts:=acts'; sb:=sb'; rmw:=rmw'; rf:=rf'; mo:=mo'; sc:=sc' |})
+  (GSTEP: gstep acts sb rmw rf mo sc acts' sb' rmw' rf' mo' sc' a a):
+  Coherent acts' sb' rmw' rf' mo' sc'.
+Proof.
+unfold new_G_write in *; ins; desf.
+
+exploit gstep_hb_write; eauto with acts.
+intro HB.
+
+assert (forall b, loc b = loc a -> loc b = Some l).
+  by ins; unfold loc in *; destruct a as [??[]]; desf.
+
+destruct WRITABLE; desc; red in SIM_TVIEW; desc; red in CUR; desc.
+specialize (CUR_UR l); specialize (CUR_RW l); specialize (CUR_SC l).
+clear SC1. (* this assumption is redundant *)
+cdes COH.
+red; splits; eauto.
+- red; ins. destruct MO as [MO1|[MO2|MO3]]; eauto 3.
+  eby red in MO3; desf; eapply FRESH; [eapply rf_acta|eapply rmw_actb].
+- red; ins; destruct MO as [MO1|MO2].
+  eapply gstep_hb_a in HB0; eauto 2.
+  eby intro; subst; eapply FRESH; eapply mo_acta.
+  red in MO2; desf.
+  eby eapply FRESH; eapply rf_acta.
+  apply HB in HB0.
+  destruct HB0 as [[HB0|HB0]|HB0].
+  eby eapply FRESH; eapply hb_actb.
+  all: eapply max_value_lt with (tm := (View.rlx (TView.cur tview))); eauto. 
+  * unfold seq, sb_ext, seq, eqv_rel, singl_rel in *; desc; subst z1 z0.
+    repeat eexists; splits; eauto.
+    right; repeat eexists; splits; eauto.
+  * unfold sb_ext, seq, eqv_rel, singl_rel in *;desc; subst z0 z.
+    repeat eexists; splits; eauto.
+    right; repeat eexists; splits; eauto.
+- red; ins; destruct MO as [MO1|MO2].
+  eapply gstep_hb_a in HB0; eauto 2.
+  eby intro; subst; eapply FRESH; eapply mo_acta.
+  red in MO2; desf; apply HB in HB0; destruct HB0 as [[?|[??]]|?]; desc.
+  all: try eby eapply FRESH; eapply hb_acta.
+  all: try eby eapply FRESH; eapply hb_actb.
+  all: try eby unfold sb_ext, seq, eqv_rel in *; desf.
+  all: unfold sb_ext, seq, eqv_rel, singl_rel in *; desc; subst z0 z.
+  all: eapply max_value_lt with (tm := (View.rlx (TView.cur tview))); eauto.
+  all: repeat eexists; splits; eauto.
+  all: left; repeat eexists; splits; eauto.
+- red; ins; apply HB in HB0; destruct HB0 as [[?|[??]]|?]; desc; 
+    try eby unfold sb_ext, seq, eqv_rel in *; desc; subst c z0; 
+    eapply FRESH; eapply rf_actb.
+  destruct MO as [?|MO]; eauto 2.
+  red in MO; desf.
+  eby eapply FRESH; eapply hb_acta.
+  eby eapply FRESH; eapply rf_acta.
+- red; ins.
+  destruct MO as [MO1|MO2]; cycle 1.
+  eby red in MO2; desf; eapply FRESH; eapply rf_acta.
+  apply HB in HB0; destruct HB0 as [[?|[??]]|?]; desc; eauto 2;
+  eby unfold sb_ext, seq, eqv_rel in *; desc; subst d z0; 
+    eapply FRESH; eapply rf_actb.
+- red; ins.
+  destruct MO as [MO1|MO2]; cycle 1.
+  eby red in MO2; desf; eapply FRESH; eapply rf_acta.
+  apply HB in HB0; destruct HB0 as [[?|[??]]|?]; desc.
+  all: try eby unfold sb_ext, seq, eqv_rel in *; desc; subst d z0 z;
+    destruct a as [??[]]; ins.
+  apply HB in HB1; destruct HB1 as [[?|[??]]|?]; desc; eauto 2.
+  all: eby unfold sb_ext, seq, eqv_rel in *; desc; subst e z0; 
+    eapply FRESH; eapply rf_actb.
+- red; ins.
+unfold union, new_mo in *; desf; eauto 2.
+all: try eby eapply FRESH; eapply rf_acta.
+all: try eby eapply FRESH; eapply rmw_actb.
+all: try eby eapply FRESH; eapply mo_actb.
+all: try eby eapply FRESH; eapply mo_acta.
+
+assert (loc a = Some l).
+by destruct a as [??[]]; ins; desf.
+
+assert(loc c = Some l /\ loc d = Some l /\ loc a0 = Some l); desc.
+red in WF; desc.
+red in WF_RMW; desc.
+splits; by apply RMW_LOC in RMW; desc; congruence.
+
+assert (exists m, Memory.get l (f_to c) memory = Some (f_to a0, m)); desc.
+eapply SIM_MEM; eauto.
+red; eauto.
+
+assert (TF: f_to a0 = f_from c).
+specialize (SIM_MEM l); desc.
+destruct m.
+exploit (SIMCELL (f_to c) (f_to a0)); try edone.
+ins; desc.
+assert (b=c); subst.
+eby cdes COH; cdes WF; eapply monotone_injective.
+done.
+
+eapply NEW_TO; splits; eauto.
+by rewrite <- TF; done.
+by eapply Time.le_lteq; eauto.
+
+- red; ins.
+  eapply gstep_hb_a in HB0; try edone; cycle 1.
+  eby intro; subst; eapply FRESH; eapply rf_actb.
+  destruct SC as [SCo|SCn]; cycle 1.
+  eby unfold sc_ext in *; desc; subst e; eapply FRESH; eapply hb_acta.
+  assert (a <> d).
+    eby intro; subst; eapply FRESH; eapply sc_acta.
+  assert (RFHBF_: b = d \/
+          (exists c, clos_refl rf' b c /\ hb acts sb rmw' rf' c d /\ is_sc_fence d)).
+    destruct RFHBF as [X|[c [RF' [HB' F]]]]; auto.
+    right; exists c; splits; try edone.
+    eapply gstep_hb_a in HB'; eauto.
+  clear RFHBF.
+  destruct MO as [?|MO]; eauto 2.
+  destruct MO; desc; subst; unfold clos_refl in *; desf; auto.
+  eby eapply FRESH; eapply hb_acta.
+  all: eby eapply FRESH; eapply rf_acta.
+- red; ins.
+
+  assert (a <> d).
+    destruct SC; unfold sc_ext in *; desc; intro; subst; eapply FRESH; try edone.
+    eby eapply sc_acta.
+
+  assert (RFHBF_: b = d \/
+          (exists c, clos_refl rf' b c /\ hb acts sb rmw' rf' c d /\ is_sc_fence d)).
+    destruct RFHBF as [X|[c [RF' [HB' F]]]]; auto.
+    right; exists c; splits; try edone.
+    eapply gstep_hb_a in HB'; eauto.
+  clear RFHBF.
+
+  assert (MO': mo a0 b \/ a0=a /\ In b acts /\ is_write b /\ 
+      loc b = loc a /\ Time.lt to (f_to b)).
+    destruct MO as [?|MO]; auto.
+    destruct MO; auto; desc; subst b.
+    exfalso; destruct RFHBF_ as [A|B]; auto; desc.
+    destruct B; try subst c.
+    eby eapply FRESH; eapply hb_acta.
+    eby eapply FRESH; eapply rf_acta.
+  clear MO.
+
+  destruct (classic (e=a)) as [EQ|NEW]; subst.
+  * destruct SC as [?|SC].
+    eby eapply FRESH; eapply sc_actb.
+    unfold sc_ext in *; desc.
+    destruct HB0 as [HB0|HB0]; cycle 1; try subst a0; desc.
+    by destruct a as [??[]]; ins.
+    destruct MO' as [?|MO]; desc.
+    eby eapply FRESH; eapply mo_acta.
+    assert (rfhbsc_opt acts sb rmw' rf' l b d).
+     by red; unfold clos_refl, eqv_rel, seq; desf; eauto 15.
+    eapply max_value_lt with (tm:= sc_map); eauto.
+    by eapply SC2; destruct a as [??[]]; unfold is_sc_wf in *; ins; desf.
+    by eexists d,d; splits; red; eauto.
+  * destruct SC as [SC|?]; cycle 1.
+    by unfold sc_ext in *; desc; subst; auto.
+    destruct HB0 as [?|HB0]; try subst a0; desc.
+    by destruct MO' as [MO'|?]; desc; eauto 3.
+    apply HB in HB0; destruct HB0 as [[?|[??]]|?]; desc.
+    + destruct MO' as [MO'|?]; desc; eauto 4.
+    eby subst a0; eapply FRESH; eapply hb_actb.
+    + unfold sb_ext, eqv_rel, seq in *; desc; subst z0 z a0.
+      destruct MO' as [?|MO']; desc.
+      eby eapply FRESH; eapply mo_acta.
+      eapply max_value_lt with (tm:= View.rlx (TView.cur tview)); eauto.
+      eexists x,x; splits.
+      left; unfold c_cur, rwr, urr, rfhbsc_opt, clos_refl, eqv_rel, seq in *; desf; eauto 30.
+      by splits; try eexists; eauto.
+    + unfold sb_ext, eqv_rel, seq in *; desc; subst z0 z a0.
+      destruct MO' as [?|MO']; desc.
+      eby eapply FRESH; eapply mo_acta.
+      eapply max_value_lt with (tm:= View.rlx (TView.cur tview)); eauto.
+      eexists e, e; splits.
+      left; unfold c_cur, rwr, urr, rfhbsc_opt, clos_refl, eqv_rel, seq in *; desf; eauto 30.
+      splits; try eexists; eauto.
+- eby eapply new_G_non_read_NoPromises.
+Qed.
+
+Lemma GMsim_write ts G tid lang st1 st2 lc1 lc2 threads sc_map mem sc_map' mem'
+  (SIM: GMsim (Configuration.mk threads sc_map mem) {| ts:= ts; exec:= G |})
+  (TID: IdentMap.find tid threads =
+        Some (existT (fun lang : Language.t => Language.state lang) lang st1, lc1))
+  l from to v released o kind
+  (STATE: Language.step lang (Some (ProgramEvent.write l v o)) st1 st2)
+  (LOCAL: Local.write_step lc1 sc_map mem l
+          from to v None released o lc2 sc_map' mem' kind):
+  exists ax_st', step {| ts:= ts; exec:= G |} ax_st' /\
+    GMsim (Configuration.mk 
+        (IdentMap.add tid (existT Language.state lang st2, lc2) threads) sc_map' mem')
+     ax_st'.
+Proof.
+generalize (fresh_id (acts G) (Some tid) (Astore l v o)); intro; desc.
+unfold GMsim, sim_time in *; desc; ins.
+assert (LOCAL':=LOCAL).
+destruct LOCAL'; ins; subst.
+
+assert (is_proper a).
+by red; eauto.
+
+assert (forall b : event, In b (acts G) /\ is_write b /\ loc b = loc a -> f_to b <> to).
+{ red; ins; desf.
+specialize (SIM_MEM l); desc.
+eapply (DOM b); splits; eauto 2 with acts.
+by destruct a as [??[]]; ins; desf.
+ destruct WRITE, PROMISE.
+* eapply Memory.add_get0; eauto.
+* eapply Memory.split_get0; eauto.
+* erewrite NO_PROMISES in PROMISES; try edone.
+eapply Memory.lower_get0 in PROMISES.
+by rewrite Memory.bot_get in *. }
+
+assert (kind = Memory.op_kind_add /\ promises2 = Memory.bot /\ exists promises0, 
+ << ADD: Memory.add mem l from to v (TView.write_released (Local.tview lc1) sc_map l to None o) mem2 >> /\
+ << REMOVE: Memory.remove promises0 l from to v (TView.write_released (Local.tview lc1) sc_map l to None o) promises2 >>).
+{  destruct WRITE, PROMISE; splits; eauto. 
+all: erewrite NO_PROMISES in PROMISES; try edone.
+all: try apply Memory.split_get0 in PROMISES.
+all: try apply Memory.lower_get0 in PROMISES.
+all: try by desc; rewrite Memory.bot_get in *.
+apply Memory.ext; ins.
+by rewrite (Memory.remove_o _ _ REMOVE), (Memory.add_o _ _ PROMISES), Memory.bot_get;
+desf; ins; desf.
+}
+
+desc; subst promises2.
+
+assert (forall b : event, In b (acts G) -> upd f_to a to b = f_to b).
+  by unfold upd; desf; ins; desf.
+
+assert (forall b : event, In b (acts G) -> upd f_from a from b = f_from b).
+  by unfold upd; desf; ins; desf.
+
+assert (MONOTONE': monotone (mo (new_G_write G a f_to to)) (upd f_to a to)).
+  by eapply new_f_to_monotone; eauto 2 with acts.
+
+assert (sim_tview f_to (acts G) (sb G) (rmw G) (rf G) (sc G) (Local.tview lc1) (thread a)).
+  by rewrite THREAD_ID in *; eapply SIM_TVIEW; eauto.
+
+exploit exists_gstep_write; eauto with acts.
+by eapply wf_new_mo_write with (to:=to); eauto 2 with acts.
+intro GSTEP.
+eapply GMsim_helper with 
+    (e:=ThreadEvent.write l from to v 
+      (TView.write_released (Local.tview lc1) sc_map l to None o) o) 
+    (tid:=tid) (f_to:=f_to) (f_to':=upd f_to a to) 
+    (f_from:=f_from) (f_from':=upd f_from a from)
+    (G':= new_G_write G a f_to to); eauto.
+* red; splits; eauto.
+* eapply write; eauto.
+  unfold get_program_event; eauto.
+  eapply new_G_write_coherent; ins; desc; eauto.
+  assert (exists v, val x = Some v); desc.
+    by destruct x as [??[]]; try exists v0; ins; desf.
+  clear MONOTONE'.
+  exploit sim_mem_get; eauto.
+  cdes COH; cdes WF; eauto.
+  intro M; desc.
+  destruct ADD, ADD.
+  eapply DISJOINT; try edone.
+  econs; ins; eauto.
+  by eapply Time.le_lteq; eauto.
+* ins.
+  rewrite IdentMap.gsspec in TID0; desf; ins; try edone.
+  pattern to at 2; erewrite <- upds with (b:=to).
+  rewrite <- THREAD_ID; eapply tview_step_write; eauto.
+* unfold new_G_write; ins.
+  pattern to at 2; erewrite <- upds with (b:=to).
+  eapply sc_map_step_write; eauto.
+* unfold new_G_write; ins.
+  eapply memory_step_write; eauto.
+  eapply WF_OP_ST.
+  rewrite !upds.
+  eby eapply MemoryFacts.MemoryFacts.write_time_lt.
+  erewrite NO_PROMISES in WRITE; try edone.
+  by rewrite !upds; desf.
+Qed.
+
+(******************************************************************************)
+(** * Lemmas for update step  *)
+(******************************************************************************)
+
+(* Lemma exists_gstep_update acts sb rmw rf mo sc a_r a_w 
+  (WF: Wf acts sb rmw rf mo sc)
+  (FRESH: ~ In a_w acts) (PROPER: is_proper a_w) (WRITE: is_write a_w)
+  (IN: In a_r acts) (TID: thread a_r = thread a_w)
+(READ: is_read a_r) (LAST: forall b, ~ sb a_r b)
+l (LOCar: loc a_r = Some l) (LOCaw: loc a_w = Some l)
+  f_to to (WF_MO': WfMO (a_w :: acts) (mo +++ new_mo acts f_to a_w to)):
+  gstep acts sb rmw rf mo sc 
+      (a_w :: acts) (sb +++ sb_ext acts a_w)
+      (rmw +++ singl_rel a_r a_w) rf (mo +++ new_mo acts f_to a_w to) (sc +++ sc_ext acts a_w) a_r a_w.
+Proof.
+red; splits; eauto.
+by unfold sb_ext, union, eqv_rel, seq; eauto 8.
+by right; splits; eauto; intro; subst.
+by unfold sc_ext, union; eauto.
+by red; unfold inclusion, union; splits; ins; eauto.
+red; splits; try done.
+- eby eapply wf_new_acts.
+- eby eapply wf_new_sb.
+- cdes WF; cdes WF_RMW.
+red; splits; unfold inclusion, union, singl_rel, sb_ext, seq, eqv_rel; splits; ins; desf; eauto 20.
+exfalso; apply FRESH; eapply sb_actb; eauto.
+
+Qed. *)
+
+(******************************************************************************)
+(** * Lemmas for fence step  *)
+(******************************************************************************)
+Definition new_G_fence G a :=
+{| acts:=(a :: acts G); sb:=(sb G +++ sb_ext (acts G) a);
+           rmw:=(rmw G) ; rf:=(rf G); mo:= (mo G);
+           sc:=(Machine.sc G +++ sc_ext (acts G) a) |}.
+
+Lemma exists_gstep_fence acts sb rmw rf mo sc a 
+  (WF: Wf acts sb rmw rf mo sc)
+  (FRESH: ~ In a acts) (PROPER: is_proper a) (FENCEa: is_fence a):
+  gstep acts sb rmw rf mo sc 
+      (a :: acts) (sb +++ sb_ext acts a)
+      rmw rf mo (sc +++ sc_ext acts a) a a.
+Proof.
+red; splits; eauto.
+by unfold sb_ext, union, eqv_rel, seq; eauto 8.
+by red; eauto.
+by unfold sc_ext, union; eauto.
+by red; unfold inclusion, union; splits; ins; eauto.
+red; splits; try done.
+- eby eapply wf_new_acts.
+- eby eapply wf_new_sb.
+- eby eapply wf_new_rmw.
+- eapply wf_new_rf; eauto 2 with acts.
+- eby eapply wf_new_mo; eauto 2 with acts.
+- eby eapply wf_new_sc.
+Qed.
+
+Lemma new_G_fence_coherent 
+  acts sb rmw rf mo sc a
+  (COH: Coherent acts sb rmw rf mo sc)
+  or ow (LABEL: lab a = Afence or ow)
+  (FRESH: ~ In a acts)
+  acts' sb' rmw' rf' mo' sc' 
+  (NEW_G: new_G_fence {| acts:=acts; sb:=sb; rmw:=rmw; rf:=rf; mo:=mo; sc:=sc |}
+   a = {| acts:=acts'; sb:=sb'; rmw:=rmw'; rf:=rf'; mo:=mo'; sc:=sc' |})
+  (GSTEP: gstep acts sb rmw rf mo sc 
+               acts' sb' rmw' rf' mo' sc' a a):
+  Coherent acts' sb' rmw' rf' mo' sc'.
+Proof.
+unfold new_G_fence in *; ins; desf.
+
+cdes COH.
+red; splits; eauto.
+- red; ins.
+eapply gstep_hb_a in HB; eauto 2.
+eby intro; subst; apply FRESH; eapply mo_acta.
+- red; ins.
+eapply gstep_hb_a in HB; eauto 2.
+eby intro; subst; apply FRESH; eapply mo_acta.
+- red; ins.
+eapply gstep_hb_a in HB; eauto 2.
+eby intro; subst; apply FRESH; eapply rf_actb.
+- red; ins.
+eapply gstep_hb_a in HB; eauto 2.
+eby intro; subst; apply FRESH; eapply rf_actb.
+
+- red; ins.
+eapply gstep_hb_a in HB; eauto 3.
+eapply gstep_hb_a in HB0; eauto 3.
+eby intro; subst; apply FRESH; eapply rf_actb.
+intro; subst d; eapply max_elt_hb; eauto.
+- red; ins.
+eapply gstep_hb_a in HB; eauto 3;
+desf; red in SC; unfold sc_ext in *; desf; eauto 3.
+all: try eby apply FRESH; eapply hb_acta.
+eapply gstep_hb_a in RFHBF0; eauto 2.
+by eapply Cscr; eauto.
+all: try eby intro; subst; apply FRESH; eapply sc_acta.
+all: try eby intro; subst; apply FRESH; eapply rf_actb.
+- red; ins.
+assert (hb (a :: acts) (sb +++ sb_ext acts a) rmw' rf' e a0 -> hb acts sb rmw' rf' e a0).
+  eapply gstep_hb_a; eauto 3.
+  eby intro; subst; apply FRESH; eapply mo_acta.
+
+assert (forall c g, sc d g /\ hb (a :: acts) (sb +++ sb_ext acts a) rmw' rf' c d ->
+  hb acts sb rmw' rf' c d).
+  ins; desc; eapply gstep_hb_a; eauto 3.
+  eby intro; subst; apply FRESH; eapply sc_acta.
+ desf; red in SC; unfold sc_ext in *; desf.
+all: try by eapply Csc; eauto 7.
+all: try eby apply FRESH; eapply mo_acta.
+all: try by eapply max_elt_hb; eauto.
+- eby eapply new_G_non_read_NoPromises.
+Qed.
+
+Lemma GMsim_fence ts G tid lang st1 st2 lc1 lc2 threads sc_map mem sc_map' 
+  (SIM: GMsim (Configuration.mk threads sc_map mem) {| ts:= ts; exec:= G |})
+  (TID: IdentMap.find tid threads =
+        Some (existT (fun lang : Language.t => Language.state lang) lang st1, lc1))
+  or ow
+  (STATE: Language.step lang (Some (ProgramEvent.fence or ow)) st1 st2)
+  (LOCAL: Local.fence_step lc1 sc_map or ow lc2 sc_map'):
+  exists ax_st', step {| ts:= ts; exec:= G |} ax_st' /\
+    GMsim (Configuration.mk 
+        (IdentMap.add tid (existT Language.state lang st2, lc2) threads) sc_map' mem)
+     ax_st'.
+Proof.
+generalize (fresh_id (acts G) (Some tid) (Afence or ow)); intro; desc.
+unfold GMsim, sim_time in *; desc; ins.
+assert (LOCAL':=LOCAL).
+destruct LOCAL'; ins; subst.
+assert (is_proper a).
+  by red; eauto.
+exploit exists_gstep_fence; eauto with acts.
+intro GSTEP.
+eapply GMsim_helper with 
+    (e:=ThreadEvent.fence or ow)
+    (tid:=tid) (f_to:=f_to) (f_to':=f_to) 
+    (f_from:=f_from) (f_from':=f_from)
+    (G':= new_G_fence G a); eauto.
+- red; splits; eauto.
+-  eapply fence; eauto.
+  unfold get_program_event; eauto.
+  eapply new_G_fence_coherent; try edone.
+- ins.
+  rewrite IdentMap.gsspec in TID0; desf; ins; try edone.
+  rewrite <- THREAD_ID.
+  destruct (classic (is_sc a));
+    [ eapply tview_step_scfence|eapply tview_step_rafence]; eauto.
+  eby  rewrite THREAD_ID in *; eapply SIM_TVIEW.
+  eby eapply WF_OP_ST.
+  eby  rewrite THREAD_ID in *; eapply SIM_TVIEW.
+- unfold new_G_fence; ins.
+  eapply sc_map_step_fence; eauto.
+  eby rewrite THREAD_ID in *; eapply SIM_TVIEW.
+- eapply memory_step_nonwrite; eauto.
+  eapply new_G_fence_coherent; eauto.
+  by eauto 3 with acts.
+Qed.
+
+(******************************************************************************)
+(** * Main theorem  *)
+(******************************************************************************)
+
+Lemma small_step_sim :
+  forall ax_st op_st (SIM: GMsim op_st ax_st) op_st' e tid
+  (OPSTEP: small_step false tid e op_st op_st'),
+  exists ax_st', (step ax_st ax_st') /\ GMsim op_st' ax_st'.
+Proof.
+ins; destruct ax_st as [ts G].
+destruct OPSTEP; destruct STEP; ins.
+by destruct STEP; ins; desf.
+inv STEP.
+- eapply GMsim_silent; edone.
+- destruct op_st; eapply GMsim_read; edone.
+- destruct op_st; eapply GMsim_write; edone.
+- admit.
+- destruct op_st; eapply GMsim_fence; edone.
+- admit.
+Admitted.
+
+(* lemma about machine step? *)
