src/axiomatic/MsimG.v
@@ -1,0 +1,605 @@
+(******************************************************************************)
+(** * Simulation between axiomatic and operational machines *)
+(******************************************************************************)
+
+Require Import Classical List Relations Peano_dec.
+Require Import Hahn.
+Require Import sflib.
+Require Import paco.
+
+Require Import Axioms.
+Require Import Basic.
+Require Import Language.
+Require Import Event.
+Require Import Time.
+Require Import Configuration.
+Require Import View.
+Require Import Cell.
+Require Import Memory.
+Require Import Thread.
+Require Import TView.
+
+Require Import Gevents.
+Require Import model.
+Require Import Gstep GstepRead GstepWrite GstepFence GstepOther.
+Require Import Machine.
+Require Import SimRel SimPreservation.
+
+Set Implicit Arguments.
+Remove Hints plus_n_O.
+
+Require Import Setoid Permutation.
+
+Hint Resolve gstep_wf gstep_inc coh_wf.
+
+Lemma foo (P Q : Prop) : P -> (P -> Q) -> P /\ Q.
+Proof. tauto. Qed.
+
+Lemma gstep_tm_to_a acts sb rmw rf mo sc acts' sb' rmw' rf' mo' sc'
+  prev a (GSTEP: gstep acts sb rmw rf mo sc acts' sb' rmw' rf' mo' sc' prev a)
+  (COH: Coherent acts sb rmw rf mo sc) 
+  tm l 
+  (TM_HB: inclusion (tm acts' sb' rmw' rf' sc' l ;; hb acts' sb' rmw' rf') (tm acts' sb' rmw' rf' sc' l))
+  (TM_MON: inclusion (tm acts sb rmw rf sc l) (tm acts' sb' rmw' rf' sc' l))
+  (TM_ACTS : forall x y, tm acts sb rmw rf sc l x y -> In y acts)
+   x (CUR: t_cur tm acts sb rmw rf sc (thread a) l x) :
+   tm acts' sb' rmw' rf' sc' l x a.
+Proof.
+red in CUR; red in CUR; desc.
+red in CUR; desc.
+unfold seq, eqv_rel in *.
+desc; subst.
+apply TM_HB; exists y; split.
+apply TM_MON; done.
+apply sb_in_hb; eapply gstep_sb; eauto.
+right; red; repeat (eexists; splits; eauto).
+Qed.
+
+(******************************************************************************)
+(** * Lemmas for the read step   *)
+(******************************************************************************)
+
+Lemma Readable_cur_tm acts sb rmw rf mo sc acts' sb' rmw' rf' mo' sc'
+  prev a (GSTEP: gstep acts sb rmw rf mo sc acts' sb' rmw' rf' mo' sc' prev a)
+  (COH: Coherent acts sb rmw rf mo sc) 
+  t f (MON: monotone mo f) l v o b (LABa: lab a = Aload l v o)
+  tm (CUR: max_value f (t_cur tm acts sb rmw rf sc (thread a) l) t) 
+  (WRITE : forall x, t_cur tm acts sb rmw rf sc (thread a) l x -> is_write x)
+  (ACTS : forall x, t_cur tm acts sb rmw rf sc (thread a) l x -> In x acts)
+  (COHERENT: forall c, mo' b c -> tm acts' sb' rmw' rf' sc' l c a -> False)
+  (TM_HB: inclusion (tm acts' sb' rmw' rf' sc' l ;; hb acts' sb' rmw' rf') 
+                    (tm acts' sb' rmw' rf' sc' l))
+  (TM_MON: inclusion (tm acts sb rmw rf sc l) (tm acts' sb' rmw' rf' sc' l))
+  (TM_DOMa: doma (tm acts sb rmw rf sc l) (fun e => loc e = Some l))
+  (TM_ACTS : forall x y, tm acts sb rmw rf sc l x y -> In y acts)
+  (RFb: rf' b a) : Time.le t (f b).
+Proof.
+assert (~ is_write a).
+  intro; unfold is_write in *; destruct (lab a); ins.
+red in CUR; desf.
+apply Time.bot_spec.
+eapply transitivity with (y:=f a_max); try done.
+cdes GSTEP; desf. 
+eapply monotone_converse with (acts:=(a :: acts)); ins; eauto using rf_acta, rf_doma.
+- by eapply rf_acta in RFb; try eassumption.
+- eapply rf_doma in RFb; eauto.
+- by destruct INam; desc; pattern a_max; eapply c_cur_doma; eauto.
+- by eapply loceq_rf in RFb; eauto; unfold loc in *; rewrite LABa in RFb.
+- rewrite gstep_non_write_mo with (mo':=mo'); eauto.
+  cdes WF'; eauto.
+- intro.
+  eapply COHERENT; eauto.
+  eapply gstep_non_write_mo with (acts:=acts) (mo:=mo); eauto.
+  eapply gstep_tm_to_a; eauto.
+Qed.
+
+Lemma Readable_msg_sc acts sb rmw rf mo sc acts' sb' rmw' rf' mo' sc'
+  prev a (GSTEP: gstep acts sb rmw rf mo sc acts' sb' rmw' rf' mo' sc' prev a)
+  (COH: Coherent acts sb rmw rf mo sc) 
+  (COH': Coherent acts' sb' rmw' rf' mo' sc') 
+  t f (MON: monotone mo f) l v o b (LABa: lab a = Aload l v o)
+  (MSG: max_value f (fun a => msg_rel scr acts sb rmw rf sc l a b) t)
+  (RFb: rf' b a) (SC: is_sc a): Time.le t (f b).
+Proof.
+assert (~ is_write a).
+  intro; unfold is_write in *; destruct (lab a); ins.
+red in MSG; desf.
+apply Time.bot_spec.
+eapply transitivity with (y:=f a_max); try done.
+cdes GSTEP. 
+eapply monotone_converse with (acts:=(a :: acts)); eauto.
+- right; eapply acta_msg_scr; eauto.
+- eapply rf_acta in RFb; eauto. rewrite <- ACT_STEP; eauto.
+- eauto with rel.
+- eapply rf_doma in RFb; eauto.
+- eauto with rel.
+- eapply loceq_rf in RFb; eauto. unfold loc in *. rewrite LABa in RFb. auto.
+- rewrite gstep_non_write_mo with (mo':=mo'); eauto.
+  rewrite <- ACT_STEP.
+  cdes WF'; eauto.
+- intro. 
+  eapply (Coherent_m_scr COH'); eauto. 
+  eapply gstep_non_write_mo with (mo:=mo); eauto.
+  eapply (gstep_msg_rel_scr_nonwrite COH GSTEP); eauto. 
+Qed.
+
+Lemma Readable_full acts sb rmw rf mo sc acts' sb' rmw' rf' mo' sc'
+  prev a (GSTEP: gstep acts sb rmw rf mo sc acts' sb' rmw' rf' mo' sc' prev a)
+  (COH: Coherent acts sb rmw rf mo sc) 
+  (COH': Coherent acts' sb' rmw' rf' mo' sc') 
+  f (MON: monotone mo f) l v o b (LABa: lab a = Aload l v o)
+  tview rel
+  (MSG: max_value f (fun a => msg_rel scr acts sb rmw rf sc l a b) (View.sc rel.(View.unwrap) l))
+  (CUR: sim_cur f acts sb rmw rf sc (TView.cur tview) (thread a))
+  (RFb: rf' b a): 
+    TView.readable tview l (f b) rel o.
+Proof.
+red in CUR; desc.
+constructor; try intro.
+-  eapply Readable_cur_tm; eauto using Coherent_urr, urr_hb, urr_mon with rel acts.
+   by eapply urr_actb; eauto.
+- eapply Readable_cur_tm; eauto using rwr_hb, rwr_mon with rel acts.
+  ins; eapply Coherent_rwr with (mo:=mo'); eauto.
+  right; splits; eauto with acts.
+  eapply rwr_actb; eauto.
+- eapply Readable_cur_tm; eauto using scr_hb, scr_mon with rel acts.
+  ins; eapply Coherent_scr_rf with (mo:=mo');  eauto with acts.
+  eapply scr_actb; eauto.
+- eapply Readable_msg_sc; eauto with acts.
+Qed.
+
+(******************************************************************************)
+(** * Lemmas for the write step   *)
+(******************************************************************************)
+
+Lemma Writable_cur_rwr acts sb rmw rf mo sc acts' sb' rmw' rf' mo' sc'
+  prev a (GSTEP: gstep acts sb rmw rf mo sc acts' sb' rmw' rf' mo' sc' prev a)
+  (COH: Coherent acts sb rmw rf mo sc) 
+  (COH': Coherent acts' sb' rmw' rf' mo' sc') 
+  t f f' (F : forall b, In b acts -> f' b = f b)
+  (MON: monotone mo' f') l v o (LABa: lab a = Astore l v o)
+  (CUR: max_value f (t_cur rwr acts sb rmw rf sc (thread a) l) t) 
+  (N_ZERO: Time.lt Time.bot (f' a)) : Time.lt t (f' a).
+Proof.
+red in CUR; desf; try done.
+eapply TimeFacts.le_lt_lt with (b:=f a_max); try done.
+cdes GSTEP.
+rewrite <- F; eauto with acts.
+eapply monotone_converse_strict with (acts:=(a :: acts)); eauto.
+- right; eauto with acts. 
+- left; done.
+- eauto with rel.
+- eauto with acts. 
+- eauto with rel.
+- unfold loc; rewrite LABa; done.
+- rewrite <- ACT_STEP.
+  cdes WF'; eauto.
+- intro.
+  eapply Coherent_rwr; eauto.
+  eapply gstep_tm_to_a; eauto.
+  eapply rwr_hb.
+  eapply rwr_mon; eauto.
+  eapply rwr_actb; eauto.
+- intro; subst; eauto with acts.
+Qed.
+
+Lemma Writable_cur_scr acts sb rmw rf mo sc acts' sb' rmw' rf' mo' sc'
+  prev a (GSTEP: gstep acts sb rmw rf mo sc acts' sb' rmw' rf' mo' sc' prev a)
+  (COH: Coherent acts sb rmw rf mo sc) 
+  (COH': Coherent acts' sb' rmw' rf' mo' sc') 
+  t f f' (F : forall b, In b acts -> f' b = f b)
+  (MON: monotone mo' f') l v o (LABa: lab a = Astore l v o)
+  (CUR: max_value f (t_cur scr acts sb rmw rf sc (thread a) l) t) 
+  (SC: is_sc a) 
+  (N_ZERO: Time.lt Time.bot (f' a)) : Time.lt t (f' a).
+Proof.
+red in CUR; desf; try done.
+eapply TimeFacts.le_lt_lt with (b:=f a_max); try done.
+cdes GSTEP.
+rewrite <- F; eauto with acts.
+eapply monotone_converse_strict with (acts:=(a :: acts)); eauto.
+- right; eauto with acts. 
+- left; done.
+- eauto with rel.
+- eauto with acts.
+- eauto with rel.
+- unfold loc; rewrite LABa; done.
+- rewrite <- ACT_STEP; cdes WF'; eauto.
+- intro.
+  eapply Coherent_scr_eq; eauto.
+  eapply gstep_tm_to_a; eauto.
+  eapply scr_hb.
+  eapply scr_mon; eauto.
+  eapply scr_actb; eauto.
+- intro; subst; eauto with acts. 
+Qed.
+
+Lemma Writable_sc_map acts sb rmw rf mo sc acts' sb' rmw' rf' mo' sc'
+  prev a (GSTEP: gstep acts sb rmw rf mo sc acts' sb' rmw' rf' mo' sc' prev a)
+  (COH: Coherent acts sb rmw rf mo sc) 
+  (COH': Coherent acts' sb' rmw' rf' mo' sc') 
+  t f f' (F : forall b, In b acts -> f' b = f b)
+  (MON: monotone mo' f') l v o (LABa: lab a = Astore l v o)
+  (SCMAP: max_value f (S_tm acts sb rmw rf l) t)
+  (SC: is_sc a) 
+  (N_ZERO: Time.lt Time.bot (f' a)) : Time.lt t (f' a).
+Proof.
+red in SCMAP; desf; try done.
+eapply TimeFacts.le_lt_lt with (b:=f a_max); try done.
+cdes GSTEP.
+rewrite <- F; eauto with acts.
+eapply monotone_converse_strict with (acts:=(a :: acts)); eauto.
+- right; eauto with acts. 
+- left; done.
+- eauto with rel.
+- eauto with acts.
+- eauto with rel.
+- unfold loc; rewrite LABa; done.
+- rewrite <- ACT_STEP; cdes WF'; eauto.
+- intro.
+  eapply Coherent_scr_eq; eauto.
+  red in INam; red in INam; desc.
+  eapply S_tm_sc with (b:=y); eauto with acts.
+  eapply S_tmr_mon; eauto.
+  apply SC_AT_END; eauto 4 with acts.
+  apply S_tmr_domb in INam; done.
+  eapply S_tmr_actb; eauto.
+  intro; subst; apply FRESH; eapply S_tmr_actb; eauto.
+- intro; subst; eauto with acts. 
+Qed.
+
+Lemma Writable_full acts sb rmw rf mo sc acts' sb' rmw' rf' mo' sc'
+  prev a (GSTEP: gstep acts sb rmw rf mo sc acts' sb' rmw' rf' mo' sc' prev a)
+  (COH: Coherent acts sb rmw rf mo sc) 
+  (COH': Coherent acts' sb' rmw' rf' mo' sc') 
+  f f' (F : forall b, In b acts -> f' b = f b)
+  (MON: monotone mo' f') (N_ZERO: Time.lt Time.bot (f' a))
+  l v o (LABa: lab a = Astore l v o)
+  tview sc_map
+  (SC : forall l : Loc.t, max_value f (S_tm acts sb rmw rf l) (sc_map l))
+  (CUR: sim_cur f acts sb rmw rf sc (TView.cur tview) (thread a)):
+  TView.writable tview sc_map l (f' a) o.
+Proof.
+red in CUR; desc.
+constructor; try intro.
+eapply Writable_cur_rwr; eauto.
+eapply Writable_cur_scr; eauto with acts.
+eapply Writable_sc_map; eauto with acts.
+Qed.
+
+(******************************************************************************)
+(** * Main Theorem: the operational machine simulates the axiomatic machine   *)
+(******************************************************************************)
+
+Definition proof_obligation ax_st G' op_st i lang st st' :=
+  forall
+   G (G_ : G = exec ax_st)
+   (COH : Coherent (acts G) (sb G) (rmw G) (rf G) (mo G) (sc G))
+   (WF_OP_ST : Configuration.wf op_st)
+   (STATES : ts ax_st = IdentMap.map fst (Configuration.threads op_st))
+   ffrom fto 
+  (TIME : sim_time (Configuration.threads op_st) (Configuration.sc op_st)
+          (Configuration.memory op_st) G ffrom fto) tview
+   j (THREAD: i = Some j)
+   (TVIEW : sim_tview fto (acts G) (sb G) (rmw G) (rf G) (sc G) tview i)
+   (LWF : TView.wf tview)
+   (SPACE : forall x y (MO: mo G x y) (NRMW: ~ (rf G ;; rmw G) x y),
+                 fto x <> ffrom y)
+   (BSPACE : forall y (INy: In y (acts G)) (W: is_write y)
+                       (NRMW: ~ exists x, (rf G ;; rmw G) x y),
+                 Time.bot <> ffrom y),
+  exists te tview' sc' mem' op_st' threads' local', 
+    << OP_ST': op_st' = Configuration.mk threads' sc' mem' >> /\ 
+    << THREAD': threads' = IdentMap.add j (existT Language.state lang st', local') 
+                                          (Configuration.threads op_st) >> /\ 
+    << LOCAL': local' = Local.mk tview' Memory.bot >> /\ 
+    << STEP: Thread.program_step te 
+                    (Thread.mk lang st (Local.mk tview Memory.bot) 
+                               (Configuration.sc op_st) (Configuration.memory op_st))
+                    (Thread.mk lang st' local' sc' mem') >> /\
+    exists ffrom' fto', 
+      << F_FROM: forall b, In b (acts G) -> ffrom' b = ffrom b >> /\
+      << F_TO: forall b, In b (acts G) -> fto' b = fto b >> /\
+      << MONOTONE: monotone (mo G') fto' >> /\  
+      << SIM_TVIEW: sim_tview fto' (acts G') (sb G') (rmw G') (rf G') (sc G') tview' i >> /\
+      << SIM_SC_MAP: forall l, max_value fto' (S_tm (acts G') (sb G') (rmw G') (rf G') l) 
+                                         (LocFun.find l sc')  >> /\
+      << SIM_MEM: sim_mem ffrom' fto' (acts G') (sb G') (rmw G') (rf G') (sc G') mem'  >> /\
+      << SPACE : forall x y (MO: mo G' x y) (NRMW: ~ (rf G' ;; rmw G') x y),
+                 fto' x <> ffrom' y >> /\
+      << BSPACE : forall y (INy: In y (acts G')) (W: is_write y)
+                       (NRMW: ~ exists x, (rf G' ;; rmw G') x y),
+                 Time.bot <> ffrom' y >>.
+
+
+Lemma ax_op_sim_step_read :
+  forall op_st ths G G' a l v o (LABa : lab a = Aload l v o)
+   (GSTEP : gstep (acts G) (sb G) (rmw G) (rf G) (mo G) (sc G) 
+          (acts G') (sb G') (rmw G') (rf G') (mo G') (sc G') a a)
+   (COH' : Coherent (acts G') (sb G') (rmw G') (rf G') (mo G') (sc G'))
+   lang st st' (STATE : Language.step lang (Some (ProgramEvent.read l v o)) st st'),
+  proof_obligation {|ts:=ths; exec:=G|} G' op_st (thread a) lang st st'.
+Proof.
+  red; ins; red in TIME; desc.
+  subst G0; destruct G, G'; simpl; ins.
+
+generalize (gstep_read_rf COH GSTEP LABa); intro; desc.
+
+assert (E: exists from rel, Memory.get l (fto b) (Configuration.memory op_st) = 
+          Some (from, Message.mk v rel) /\ sim_mem_helper fto acts sb rmw rf sc b from v rel.(View.unwrap)).
+{ cdes COH; cdes WF.
+  by eexists; eapply sim_mem_get; eauto with acts; destruct b as [??[]]; ins; desf.
+}
+
+desc; red in E0; desc.
+
+assert (WRITE_B: is_write b). 
+  unfold is_write; destruct (lab b); ins.
+assert (LOC_B: Gevents.loc b = Some l). 
+  unfold Gevents.loc; destruct (lab b); ins; desf.
+
+eexists _,_,_,_,_,_,_.
+splits; eauto.
+- eapply Thread.step_read; eauto.
+  econstructor; eauto.
+  red in TVIEW; red in SIMMSG; desc.
+  eapply Readable_full;eauto. 
+- exists ffrom, fto; splits; eauto.
+  * rewrite <- gstep_non_write_mo; eauto with acts.
+  * eapply tview_step_read with (acts := acts) (acts0 := acts0); eauto.
+  * ins. eapply max_value_same_set; try edone.
+    ins; rewrite gstep_S_tm_other; eauto with acts.
+  * eapply memory_step_nonwrite with (acts := acts) (acts0 := acts0); eauto with acts.
+  * ins; eapply SPACE.
+      by eapply gstep_mo; eauto; intro; subst; 
+         [eapply mo_doma in MO|eapply mo_domb in MO]; 
+         eauto; destruct a as [??[]].
+    intro X; apply (gstep_rf_rmw_nonwrite COH GSTEP) in X; eauto;
+    by destruct a as [??[]].
+  * cdes GSTEP; subst; ins; desf; [by destruct y as [??[]]|].
+    apply BSPACE; eauto; intro; desc; apply NRMW; eexists.
+    eapply seq_mori; eauto using rf_mon, rmw_mon.
+Qed.
+
+Lemma ax_op_sim_step_write :
+  forall op_st ths G G' a l v o (LABa : lab a = Astore l v o)
+   (GSTEP : gstep (acts G) (sb G) (rmw G) (rf G) (mo G) (sc G) 
+      (acts G') (sb G') (rmw G') (rf G') (mo G') (sc G') a a)
+   (COH' : Coherent (acts G') (sb G') (rmw G') (rf G') (mo G') (sc G')) 
+   lang st st' (STATE : Language.step lang (Some (ProgramEvent.write l v o)) st st'),
+  proof_obligation {|ts:=ths; exec:=G|} G' op_st (thread a) lang st st'.
+Proof.
+  red; ins; red in TIME; ins; desc.
+  subst G0; destruct G, G'; simpl; ins.
+
+  edestruct new_f with (dom := fun l x => In x acts0 /\ is_write x /\ loc x = Some l) 
+                       (a:=a) (acts:=acts) (mo := mo0) (f_to := fto) (f_from:=ffrom)
+    as (f_from' & L); desc;
+    try eassumption;
+    try (by cdes GSTEP; ins; apply WF'). 
+    ins; cdes GSTEP; cdes WF'; cdes WF_MO.
+    exploit MO_ACTa; eauto; exploit MO_DOMa; eauto.
+    exploit MO_ACTb; eauto; exploit MO_DOMb; eauto.
+    by exploit MO_LOC; eauto; ins; desf; eauto 10.
+    by ins; desf.
+    by cdes GSTEP; subst; intros; desf.
+    by cdes GSTEP; red; ins; eapply MONOTONE, gstep_mo; eauto; congruence.
+    {
+      ins; eapply SPACE. 
+        cdes GSTEP; eapply gstep_mo; eauto;
+        by try intro; subst; cdes WF'; eapply WF_MO; eauto.
+      unfold seq; intro; desc.  
+      eapply rf_mon in H; eauto.
+      eapply rmw_mon in H0; eauto.
+      by cdes COH'; eapply Cat with (a:= x) (b:= a) (c := y); eauto. 
+    }
+    {
+      ins; exploit mo_actb; try exact MO; eauto.
+      exploit mo_domb; try exact MO; eauto.
+      intros K K'; cdes GSTEP; desf; ins; desf.
+        by cdes WF'; exfalso; eapply WF_MO; eauto.
+      destruct (classic (exists x : event, (rf;; rmw) x y)) as [C|]; desc; eauto.
+      assert (INx: In x acts).
+        by eapply seq_doma in C; [|eapply rf_acta]; eauto. 
+      assert (NEQ: x <> a) by congruence.
+      eapply seq_mori in C; eauto using rf_mon, rmw_mon.
+      assert (IMM': immediate mo0 x y).
+        split; [by eapply rf_rmw_mo in C; eauto|].
+        red in C; desc; intros; cdes COH'; eapply Cat;
+        try exact C; try exact C0; eauto.
+      clear C; destruct IMM' as [C IMM'].
+      cdes WF'; cdes WF_MO. 
+        exploit (MO_LOC a y); eauto; intro; desc.
+        exploit (MO_LOC x y); eauto; intro; desf.
+      eapply WF_MO in NEQ; splits; eauto 3 with acts.
+      exfalso; des; eauto.
+    }
+    by ins; desc; eapply sim_mem_lt; eauto.
+    by ins; desc; eapply sim_mem_disj; eauto.
+
+  assert (FROM: Time.lt (f_from' a) (f_to' a)).
+  by cdes GSTEP; desf; eapply TWF; splits; auto using in_eq; 
+     destruct a as [??[]]; ins; desf.
+
+  assert (exists mem', Memory.write Memory.bot
+                        (Configuration.memory op_st) l (f_from' a) (f_to' a) v
+                        (TView.write_released tview op_st.(Configuration.sc) l (f_to' a) None o)
+                        Memory.bot mem' Memory.op_kind_add).
+  {
+    eapply memory_exists_write; try edone; ins.
+    by destruct WF_OP_ST; done.
+    red in TVIEW; desc.
+    red in CUR; desc.
+    specialize (CUR_RW l). 
+    red in CUR_RW; unfold LocFun.find in CUR_RW; desf.
+      by rewrite MAX0; eauto using Time.bot_spec.
+    etransitivity; try eapply LB'. 
+    rewrite <- F_TO, Time.le_lteq; eauto using acts_cur_rwr; left.
+    destruct (classic (a_max = a)) as [|N]; subst.
+      by exfalso; apply GSTEP; eauto using acts_cur_rwr.
+    {
+      assert (mo0 a_max a \/ mo0 a a_max); des; eauto.
+        eapply GSTEP with (l:=l); cdes GSTEP; ins; subst.
+          by splits; eauto using in_eq, in_cons, acts_cur_rwr with rel.
+        by splits; eauto 3 using in_eq, in_cons, acts_cur_rwr with rel;
+           destruct a as [??[]]; ins; desf.
+      unfold t_cur, c_cur, dom_rel, seq, eqv_rel in INam; desc; subst. 
+      exfalso; eapply (Coherent_rwr_sb COH'); eauto. 
+        by eapply rwr_mon; eauto.
+      eapply gstep_sb; eauto.
+      unfold sb_ext, union, seq, eqv_rel; eauto.
+      eauto_red 10 using rwr_actb.
+    }
+    {
+      desf; specialize (SIM_MEM l); desc.
+      destruct msg2; eapply SIMCELL in H; desf.
+      rewrite <- F_TO, <- F_FROM; ins.
+      cdes GSTEP; desf; simpls.
+      eapply DJ'; eauto; splits; eauto; try congruence;
+      destruct a as [??[]]; ins; desf.
+    }
+  }
+  desc; eexists _,_,_,mem',_,_,_; splits; eauto.
+  - eapply Thread.step_write; eauto.
+    econstructor; eauto.
+    cdes GSTEP; desf; red in TVIEW; desc; eapply Writable_full; 
+    eauto using TimeFacts.le_lt_lt, Time.bot_spec, in_eq.
+  - exists f_from', f_to'; splits; try done.
+    * eapply tview_step_write; eauto.
+    * eapply sc_map_step_write; eauto.
+    * eapply memory_step_write; eauto.
+      destruct WF_OP_ST; done.
+    * clear H.
+      cdes GSTEP; ins; subst.
+      exploit mo_acta; try exact MO; try eassumption.
+      exploit mo_actb; try exact MO; try eassumption.
+      ins; desf; subst.
+        eby intro X; rewrite X in *; eapply Time.lt_strorder. 
+        by eapply NADJ_R; eauto.
+        by eapply NADJ_L; eauto.
+      rewrite F_FROM, F_TO; ins. 
+      eapply SPACE; eauto.
+      eapply gstep_mo; eauto; try congruence.
+      by intro X; apply NRMW, (gstep_rf_rmw COH GSTEP); vauto.
+    * clear H; cdes GSTEP; subst; ins; desf. 
+      rewrite F_FROM; ins.
+      apply BSPACE; eauto; intro; desc; apply NRMW; eexists.
+      eapply seq_mori; eauto using rf_mon, rmw_mon.
+Qed.
+
+Lemma ax_op_sim_step_update :
+  forall op_st ths G G'
+         a_r l v_r o_r (LABar : lab a_r = Aload l v_r o_r)
+         a_w v_w o_w (LABaw : lab a_w = Astore l v_w o_w)
+         G_mid
+  (GSTEPr : gstep (acts G) (sb G) (rmw G) (rf G) (mo G) (sc G) 
+              (acts G_mid) (sb G_mid) (rmw G_mid) (rf G_mid)  (mo G_mid) (sc G_mid) a_r a_r)
+  (GSTEPw : gstep (acts G_mid) (sb G_mid) (rmw G_mid) (rf G_mid) (mo G_mid) (sc G_mid) 
+            (acts G') (sb G') (rmw G') (rf G') (mo G') (sc G') a_r a_w)
+  (COHmid : Coherent (acts G_mid) (sb G_mid) (rmw G_mid) (rf G_mid) (mo G_mid) (sc G_mid))
+  (COH' : Coherent (acts G') (sb G') (rmw G') (rf G') (mo G') (sc G'))
+   lang st st'
+   (STATE : Language.step lang (Some (ProgramEvent.update l v_r v_w o_r o_w)) st st'),
+  proof_obligation {|ts:=ths; exec:=G|} G' op_st (thread a_r) lang st st'.
+Proof.
+Admitted. (* updates *)
+
+Lemma ax_op_sim_step_fence :
+  forall op_st ths G G'
+         a o_r o_w (LABa : lab a = Afence o_r o_w)
+   (GSTEP : gstep (acts G) (sb G) (rmw G) (rf G) (mo G) (sc G) 
+            (acts G') (sb G') (rmw G') (rf G') (mo G') (sc G') a a)
+   (COH' : Coherent (acts G') (sb G') (rmw G') (rf G') (mo G') (sc G')) 
+   lang st st'
+   (STATE : Language.step lang (Some (ProgramEvent.fence o_r o_w)) st st'),
+  proof_obligation {|ts:=ths; exec:=G|} G' op_st (thread a) lang st st'.
+Proof.
+  ins; red; ins; red in TIME; ins; desc.
+  subst G0; destruct G, G'; simpl; ins.
+  eexists _,_,_,_,_,_,_; splits; eauto.
+  eapply Thread.step_fence; eauto.
+  econstructor; eauto.
+  exists ffrom, fto; splits; eauto.
+  * rewrite <- gstep_non_write_mo; eauto with acts.
+  * destruct (classic (is_sc a)); 
+      [ eapply tview_step_scfence|eapply tview_step_rafence]; eauto.
+  * eby eapply sc_map_step_fence.
+  * by eapply memory_step_nonwrite; eauto with acts.
+  * ins; eapply SPACE.
+      by eapply gstep_mo; eauto; intro; subst; 
+         [eapply mo_doma in MO|eapply mo_domb in MO]; 
+         eauto; destruct a as [??[]].
+    intro X; apply (gstep_rf_rmw_nonwrite COH GSTEP) in X; eauto;
+    by destruct a as [??[]].
+  * cdes GSTEP; subst; ins; desf; [by destruct y as [??[]]|].
+    apply BSPACE; eauto; intro; desc; apply NRMW; eexists.
+    eapply seq_mori; eauto using rf_mon, rmw_mon.
+Qed.
+
+Lemma find_mapD A B tid (f: A -> B) x y :
+  IdentMap.find tid (IdentMap.map f x) = Some y ->
+  exists z, IdentMap.find tid x = Some z /\ y = f z.
+Proof.
+  rewrite IdentMap.Facts.map_o; unfold option_map; ins; desf; eauto.
+Qed.
+
+Lemma ax_op_sim :
+  forall op_st ax_st (SIM: sim op_st ax_st) ax_st' (AXSTEP: step ax_st ax_st'),
+  exists e tid op_st', Configuration.step e tid op_st op_st' /\ sim op_st' ax_st'.
+Proof.
+  ins; red in SIM; desc.
+  destruct AXSTEP.
+
+  rewrite STATES in TID.
+  apply find_mapD in TID; desc; destruct z as [? local]; ins; desf.
+  destruct local as [tview promises].
+  assert (TID' := TID).
+  apply NO_PROMISES in TID'; ins; subst.
+
+  cut (proof_obligation ax_st (exec ax_st') op_st (Some i) lang st st').
+  {
+    intro X; exploit X; eauto; clear X; ins; desc.
+       by eapply TIME; eauto.
+       by destruct WF_OP_ST; destruct WF; eapply THREADS; eauto.
+    eexists _,i,_.
+    apply foo; [|intro CSTEP].
+  -  econstructor; try edone; try apply Thread.step_program; eauto.
+     red; ins; eexists; splits; eauto; simpl; desf.
+  - red; simpl; splits; eauto.
+    * destruct MSTEP; eauto.
+      by rewrite SAME_EXEC.
+    * eapply Configuration.step_future; eauto.
+      eby eapply no_promises_consistent.
+    * intro; rewrite IdentMap.gsspec. ins; desf; simpl; eapply NO_PROMISES; eauto.
+    * by rewrite IdentMap.map_add; simpl; rewrite MTS, STATES.
+    * red in TIME; desc; exists ffrom', fto'; splits; eauto. 
+      red; simpl; splits; eauto; ins.
+      rewrite IdentMap.gsspec in TID0; desf; ins; simpl.
+      destruct MSTEP; subst.
+        rewrite SAME_EXEC.
+        eapply sim_tview_other_threads_silent; eauto.
+      all: eapply sim_tview_other_threads; eauto 2.
+      all: try eapply sim_tview_other_threads; eauto 2.
+      all: try intro; subst; eauto.
+      all: congruence.
+   }
+  clear f_from f_to TIME SPACE BSPACE.
+
+  destruct MSTEP; ins; subst.
+  { (** SILENT **)
+    destruct ax_st, ax_st'; ins; desf.
+    red; ins; eexists _,_,_,_,_,_,_.
+    splits; eauto.
+    eapply Thread.step_silent; eauto.
+    red in TIME; ins; desc; subst.
+    exists ffrom, fto; splits; eauto.
+  }
+all: try rewrite <- TIDa; try rewrite <- TIDar; try rewrite <- TIDaw.
+  by eapply ax_op_sim_step_read; eauto.
+  by eapply ax_op_sim_step_write; eauto.
+  by eapply ax_op_sim_step_update; eauto.
+  by eapply ax_op_sim_step_fence; eauto.
+admit. (** SYSTEM_CALL **)
+Admitted.
+
+
